feat: theory maps

HoTTLean/Syntax/Axioms.lean
@@ -12,7 +12,24 @@ def empty (χ) : Axioms χ := fun _ => none
 
 theorem empty_wf (χ) : (empty χ).Wf := nofun
 
-open Classical
+section
+variable [DecidableEq χ]
+
+/- Remark: we require `E c = none` because it is convenient to have around later.
+We do not require `E ∣ [] ⊢[l] A` so that `@[reflect]` doesn't have to prove it. -/
+def snoc (E : Axioms χ)
+    (l : Nat) (c : χ) (A : Expr χ)
+    (l_le : l ≤ univMax) (_Ec : E c = none) (A_cl : A.isClosed) : Axioms χ :=
+  fun d => if d = c then some ⟨(A, l), ⟨A_cl, l_le⟩⟩ else E d
+
+@[simp]
+theorem snoc_get (E : Axioms χ) (l c A l_le Ec A_cl) :
+    E.snoc l c A l_le Ec A_cl c = some ⟨(A, l), ⟨A_cl, l_le⟩⟩ := by
+  simp [snoc]
+
+end
+
+/-! ## Theory inclusions -/
 
 instance : LE (Axioms χ) where
   le E E' := ∀ ⦃c p⦄, (E c) = some p → (E' c) = some p
@@ -25,77 +42,124 @@ instance : IsTrans (Axioms χ) (· ≤ ·) where
 
 theorem empty_le (E : Axioms χ) : empty χ ≤ E := nofun
 
-noncomputable def snoc (E : Axioms χ)
-    (l : Nat) (c : χ) (A : Expr χ)
-    (l_le : l ≤ univMax) (A_cl : A.isClosed) : Axioms χ :=
-  fun d => if d = c then some ⟨(A, l), ⟨A_cl, l_le⟩⟩ else E d
+theorem eq_none_of_le {E E' : Axioms χ} (le : E ≤ E') {c} (E'c : E' c = none) : E c = none := by
+  apply Option.eq_none_iff_forall_ne_some.mpr
+  intro _ h
+  simp [le h] at E'c
 
-@[simp]
-theorem snoc_get (E : Axioms χ) (l c A l_le A_cl) :
-    E.snoc l c A l_le A_cl c = some ⟨(A, l), ⟨A_cl, l_le⟩⟩ := by
-  simp [snoc]
+section
+variable [DecidableEq χ] {𝕋 𝕋' : Axioms χ} (le : 𝕋 ≤ 𝕋')
 
-theorem le_snoc {E E' : Axioms χ} (le : E ≤ E') (l c A l_le A_cl) (Ec : E c = none) :
-    E ≤ E'.snoc l c A l_le A_cl := by
-  intro d Al Ed
-  have : d ≠ c := by grind
-  simpa [snoc, this, ↓reduceIte] using le Ed
+include le in
+theorem le_snoc (l c A l_le 𝕋'c A_cl) : 𝕋 ≤ 𝕋'.snoc l c A l_le 𝕋'c A_cl := by
+  intro d Al 𝕋d
+  have : d ≠ c := fun h => nomatch (h ▸ le 𝕋d) ▸ 𝕋'c
+  simpa [snoc, this, ↓reduceIte] using le 𝕋d
 
-theorem le_snoc_self (E : Axioms χ) (l c A l_le A_cl) (Ec : E c = none) :
-    E ≤ E.snoc l c A l_le A_cl :=
-  le_snoc (refl _) l c A l_le A_cl Ec
-
-theorem snoc_le {E E' : Axioms χ} (le : E ≤ E') (l c A l_le A_cl)
-    (E'c : E' c = some ⟨(A, l), ⟨A_cl, l_le⟩⟩) :
-    E.snoc l c A l_le A_cl ≤ E' := by
-  intro d Al Ed
+include le in
+theorem snoc_le (l c A l_le 𝕋c A_cl) (𝕋'c : 𝕋' c = some ⟨(A, l), ⟨A_cl, l_le⟩⟩) :
+    𝕋.snoc l c A l_le 𝕋c A_cl ≤ 𝕋' := by
+  intro d Al 𝕋d
   by_cases eq : d = c
-  . cases eq; convert E'c using 2; simpa [snoc] using Ed.symm
-  . simp only [snoc, eq, ↓reduceIte] at Ed; exact le Ed
+  . cases eq; convert 𝕋'c using 2; simpa [snoc] using 𝕋d.symm
+  . simp only [snoc, eq, ↓reduceIte] at 𝕋d; exact le 𝕋d
 
-theorem of_le_all {E E' : Axioms χ} (le : E ≤ E') :
-    (∀ {Γ}, WfCtx E Γ → WfCtx E' Γ) ∧
-    (∀ {Γ l A}, E ∣ Γ ⊢[l] A → E' ∣ Γ ⊢[l] A) ∧
-    (∀ {Γ l A B}, E ∣ Γ ⊢[l] A ≡ B → E' ∣ Γ ⊢[l] A ≡ B) ∧
-    (∀ {Γ l A t}, E ∣ Γ ⊢[l] t : A → E' ∣ Γ ⊢[l] t : A) ∧
-    (∀ {Γ l A t u}, E ∣ Γ ⊢[l] t ≡ u : A → E' ∣ Γ ⊢[l] t ≡ u : A) := by
-  mutual_induction WfCtx
-  case ax =>
-    intros; rename_i Ec _ Γ ihA
-    apply WfTm.ax Γ (le Ec) ihA
-  grind_cases
+theorem le_snoc_self (𝕋 : Axioms χ) (l c A l_le 𝕋c A_cl) :
+    𝕋 ≤ 𝕋.snoc l c A l_le 𝕋c A_cl :=
+  le_snoc (refl _) l c A l_le 𝕋c A_cl
 
+include le in
+theorem snoc_le_snoc (l c A l_le 𝕋'c A_cl) :
+    𝕋.snoc l c A l_le (eq_none_of_le le 𝕋'c) A_cl ≤ 𝕋'.snoc l c A l_le 𝕋'c A_cl := by
+  simp [snoc_le (le_snoc le ..)]
+
+end
 end Axioms
 
-theorem WfCtx.of_axioms_le {E E' : Axioms χ} {Γ} (le : E ≤ E') (Γwf : WfCtx E Γ) :
-    WfCtx E' Γ :=
-  Axioms.of_le_all le |>.1 Γwf
+/-! ## Theory maps (translations) -/
 
-theorem WfTp.of_axioms_le {E E' : Axioms χ} {Γ A l} (le : E ≤ E') (ΓA : E ∣ Γ ⊢[l] A) :
-    E' ∣ Γ ⊢[l] A :=
-  Axioms.of_le_all le |>.2.1 ΓA
+variable {χ χ' : Type*} {𝕋 : Axioms χ} {f : χ → χ'} {𝕋' : Axioms χ'}
 
-theorem EqTp.of_axioms_le {E E' : Axioms χ} {Γ A B l} (le : E ≤ E') (ΓAB : E ∣ Γ ⊢[l] A ≡ B) :
-    E' ∣ Γ ⊢[l] A ≡ B :=
-  Axioms.of_le_all le |>.2.2.1 ΓAB
+/-- A map `f` of signatures is well-formed as a map of theories
+when it preserves the types of those base constants
+that are present in the domain. -/
+structure WfTheoryMap (𝕋 : Axioms χ) (f : χ → χ') (𝕋' : Axioms χ') : Prop where
+  get_eq (c : χ) (h : (𝕋 c).isSome) :
+    𝕋' (f c) = (𝕋 c).map fun ⟨(A, l), h⟩ => ⟨(A.map f, l), by simp [h]⟩
 
-theorem WfTm.of_axioms_le {E E' : Axioms χ} {Γ A t l} (le : E ≤ E') (Γt : E ∣ Γ ⊢[l] t : A) :
-    E' ∣ Γ ⊢[l] t : A :=
-  Axioms.of_le_all le |>.2.2.2.1 Γt
+theorem WfTheoryMap.of_le {𝕋 𝕋' : Axioms χ} (le : 𝕋 ≤ 𝕋') : WfTheoryMap 𝕋 id 𝕋' :=
+  ⟨by
+    intro _ 𝕋c
+    simp [le <| Option.eq_some_of_isSome 𝕋c]⟩
 
-theorem EqTm.of_axioms_le {E E' : Axioms χ} {Γ A t u l} (le : E ≤ E') (Γtu : E ∣ Γ ⊢[l] t ≡ u : A) :
-    E' ∣ Γ ⊢[l] t ≡ u : A :=
-  Axioms.of_le_all le |>.2.2.2.2 Γtu
+section
+variable (H : WfTheoryMap 𝕋 f 𝕋') {Γ l A B t u}
+include H
 
-theorem Axioms.Wf.snoc {E : Axioms χ} {A l}
-    (Ewf : E.Wf) (c : χ) (Awf : E ∣ [] ⊢[l] A) (Ec : E c = none) :
-    (E.snoc l c A Awf.le_univMax Awf.isClosed).Wf := by
-  intro d Al Ed
-  simp only [Axioms.snoc] at Ed
-  have le := E.le_snoc_self l c A Awf.le_univMax Awf.isClosed Ec
-  by_cases eq : d = c <;> simp only [eq, ↓reduceIte] at Ed
-  . cases Ed
+private theorem map_all :
+    (∀ {Γ}, WfCtx 𝕋 Γ → WfCtx 𝕋' (Γ.map f)) ∧
+    (∀ {Γ l A}, 𝕋 ∣ Γ ⊢[l] A → 𝕋' ∣ Γ.map f ⊢[l] A.map f) ∧
+    (∀ {Γ l A B}, 𝕋 ∣ Γ ⊢[l] A ≡ B → 𝕋' ∣ Γ.map f ⊢[l] A.map f ≡ B.map f) ∧
+    (∀ {Γ l A t}, 𝕋 ∣ Γ ⊢[l] t : A → 𝕋' ∣ Γ.map f ⊢[l] t.map f : A.map f) ∧
+    (∀ {Γ l A t u}, 𝕋 ∣ Γ ⊢[l] t ≡ u : A → 𝕋' ∣ Γ.map f ⊢[l] t.map f ≡ u.map f : A.map f) := by
+  mutual_induction WfCtx
+  case ax =>
+    intro _ _ Al _ 𝕋c _ _
+    apply WfTm.ax (Al := ⟨(Al.1.1.map f, Al.1.2), by simp [Al.2]⟩)
+    . assumption
+    . apply 𝕋c ▸ H.get_eq _ (Option.isSome_iff_exists.mpr ⟨_, 𝕋c⟩)
+  case bvar =>
+    introv _ lk _
+    apply WfTm.bvar ‹_› (lk.map f)
+
+  all_goals (
+    dsimp [Expr.map]; intros
+    try simp only [Expr.subst_map, ← Expr.up_map_comp, ← Expr.snoc_map_comp, ← Expr.map_toSb] at *)
+  case lam_app' => apply EqTm.lam_app; assumption
+  case idRec_refl' => apply EqTm.idRec_refl <;> assumption
+  case cong_idRec' => apply EqTm.cong_idRec <;> assumption
+  case cong_snd' => apply EqTm.cong_snd <;> assumption
+  case idRec' => apply WfTm.idRec <;> assumption
+  case snd' => apply WfTm.snd; assumption
+  grind_cases
+
+theorem WfCtx.map (W : WfCtx 𝕋 Γ) : WfCtx 𝕋' (Γ.map f) := (map_all H).1 W
+theorem WfTp.map (W : 𝕋 ∣ Γ ⊢[l] A) : 𝕋' ∣ Γ.map f ⊢[l] A.map f := (map_all H).2.1 W
+theorem EqTp.map (W : 𝕋 ∣ Γ ⊢[l] A ≡ B) : 𝕋' ∣ Γ.map f ⊢[l] A.map f ≡ B.map f :=
+  (map_all H).2.2.1 W
+theorem WfTm.map (W : 𝕋 ∣ Γ ⊢[l] t : A) : 𝕋' ∣ Γ.map f ⊢[l] t.map f : A.map f :=
+  (map_all H).2.2.2.1 W
+theorem EqTm.map (W : 𝕋 ∣ Γ ⊢[l] t ≡ u : A) : 𝕋' ∣ Γ.map f ⊢[l] t.map f ≡ u.map f : A.map f :=
+  (map_all H).2.2.2.2 W
+
+end
+
+section
+variable {𝕋 𝕋' : Axioms χ} (le : 𝕋 ≤ 𝕋') {Γ l A B t u}
+include le
+
+theorem WfCtx.of_axioms_le (Γwf : WfCtx 𝕋 Γ) : WfCtx 𝕋' Γ := by
+  simpa using Γwf.map (WfTheoryMap.of_le le)
+theorem WfTp.of_axioms_le (ΓA : 𝕋 ∣ Γ ⊢[l] A) : 𝕋' ∣ Γ ⊢[l] A := by
+  simpa using ΓA.map (WfTheoryMap.of_le le)
+theorem EqTp.of_axioms_le (ΓAB : 𝕋 ∣ Γ ⊢[l] A ≡ B) : 𝕋' ∣ Γ ⊢[l] A ≡ B := by
+  simpa using ΓAB.map (WfTheoryMap.of_le le)
+theorem WfTm.of_axioms_le (Γt : 𝕋 ∣ Γ ⊢[l] t : A) : 𝕋' ∣ Γ ⊢[l] t : A := by
+  simpa using Γt.map (WfTheoryMap.of_le le)
+theorem EqTm.of_axioms_le (Γtu : 𝕋 ∣ Γ ⊢[l] t ≡ u : A) : 𝕋' ∣ Γ ⊢[l] t ≡ u : A := by
+  simpa using Γtu.map (WfTheoryMap.of_le le)
+
+end
+
+theorem Axioms.Wf.snoc [DecidableEq χ] {𝕋 : Axioms χ} {A l}
+    (𝕋wf : 𝕋.Wf) (c : χ) (Awf : 𝕋 ∣ [] ⊢[l] A) (𝕋c : 𝕋 c = none) :
+    (𝕋.snoc l c A Awf.le_univMax 𝕋c Awf.isClosed).Wf := by
+  intro d Al 𝕋d
+  simp only [Axioms.snoc] at 𝕋d
+  have le := 𝕋.le_snoc_self l c A Awf.le_univMax 𝕋c Awf.isClosed
+  by_cases eq : d = c <;> simp only [eq, ↓reduceIte] at 𝕋d
+  . cases 𝕋d
     exact Awf.of_axioms_le le
-  . exact (Ewf Ed).of_axioms_le le
+  . exact (𝕋wf 𝕋d).of_axioms_le le
 
 end SynthLean
